<?xml version="1.0"?>


<!DOCTYPE rdf:RDF [
    <!ENTITY cc "http://creativecommons.org/ns#" >
    <!ENTITY owl "http://www.w3.org/2002/07/owl#" >
    <!ENTITY dc "http://purl.org/dc/elements/1.1#" >
    <!ENTITY xsd "http://www.w3.org/2001/XMLSchema#" >
    <!ENTITY owl2xml "http://www.w3.org/2006/12/owl2-xml#" >
    <!ENTITY rdfs "http://www.w3.org/2000/01/rdf-schema#" >
    <!ENTITY rdf "http://www.w3.org/1999/02/22-rdf-syntax-ns#" >
    <!ENTITY oboe-core "http://ecoinformatics.org/oboe/oboe.1.0/oboe-core.owl#" >
]>


<rdf:RDF xmlns="http://ecoinformatics.org/oboe/oboe.1.0/oboe-ecology.owl#"
     xml:base="http://ecoinformatics.org/oboe/oboe.1.0/oboe-ecology.owl"
     xmlns:dc="http://purl.org/dc/elements/1.1#"
     xmlns:rdfs="http://www.w3.org/2000/01/rdf-schema#"
     xmlns:owl2xml="http://www.w3.org/2006/12/owl2-xml#"
     xmlns:oboe-core="http://ecoinformatics.org/oboe/oboe.1.0/oboe-core.owl#"
     xmlns:owl="http://www.w3.org/2002/07/owl#"
     xmlns:xsd="http://www.w3.org/2001/XMLSchema#"
     xmlns:rdf="http://www.w3.org/1999/02/22-rdf-syntax-ns#"
     xmlns:cc="http://creativecommons.org/ns#">
    <owl:Ontology rdf:about="http://ecoinformatics.org/oboe/oboe.1.0/oboe-ecology.owl">
        <rdfs:label>OBOE Ecology</rdfs:label>
        <rdfs:comment>Copyright (c) 2006-2011 The Regents of the University of California.  All rights reserved. This work is licensed under the Creative Commons Attribution 3.0 Unported License. To view a copy of this license, visit http://creativecommons.org/licenses/by/3.0/ or send a letter to Creative Commons, 444 Castro Street, Suite 900, Mountain View, California, 94041, USA.</rdfs:comment>
        <rdfs:comment>This ontology contains ecological terms that are common across OBOE extensions.  It is not comprehensive, but rather the beginnings of a general ecological ontology.</rdfs:comment>
        <owl:versionInfo>Version 1.0</owl:versionInfo>
        <owl:imports rdf:resource="http://ecoinformatics.org/oboe/oboe.1.0/oboe-core.owl"/>
    </owl:Ontology>
    


    <!-- 
    ///////////////////////////////////////////////////////////////////////////////////////
    //
    // Annotation properties
    //
    ///////////////////////////////////////////////////////////////////////////////////////
     -->

    <owl:AnnotationProperty rdf:about="&dc;description"/>
    


    <!-- 
    ///////////////////////////////////////////////////////////////////////////////////////
    //
    // Datatypes
    //
    ///////////////////////////////////////////////////////////////////////////////////////
     -->

    


    <!-- 
    ///////////////////////////////////////////////////////////////////////////////////////
    //
    // Classes
    //
    ///////////////////////////////////////////////////////////////////////////////////////
     -->

    


    <!-- http://ecoinformatics.org/oboe/oboe.1.0/oboe-ecology.owl#AirSample -->

    <owl:Class rdf:about="http://ecoinformatics.org/oboe/oboe.1.0/oboe-ecology.owl#AirSample">
        <rdfs:label>Air Sample</rdfs:label>
        <rdfs:subClassOf rdf:resource="http://ecoinformatics.org/oboe/oboe.1.0/oboe-ecology.owl#Sample"/>
    </owl:Class>
    


    <!-- http://ecoinformatics.org/oboe/oboe.1.0/oboe-ecology.owl#BeachHabitat -->

    <owl:Class rdf:about="http://ecoinformatics.org/oboe/oboe.1.0/oboe-ecology.owl#BeachHabitat">
        <rdfs:label>Beach Habitat</rdfs:label>
        <rdfs:subClassOf rdf:resource="http://ecoinformatics.org/oboe/oboe.1.0/oboe-ecology.owl#EcologicalHabitat"/>
        <rdfs:comment>This habitat should have an object property that ties it to a Beach environment </rdfs:comment>
        <rdfs:comment>TO DO MOB: find similarConceptTo</rdfs:comment>
    </owl:Class>
    


    <!-- http://ecoinformatics.org/oboe/oboe.1.0/oboe-ecology.owl#EcologicalCommunity -->

    <owl:Class rdf:about="http://ecoinformatics.org/oboe/oboe.1.0/oboe-ecology.owl#EcologicalCommunity">
        <rdfs:label>Ecological Community</rdfs:label>
        <rdfs:subClassOf rdf:resource="&oboe-core;Entity"/>
        <dc:description>In ecology, a community is an assemblage of two or more populations of different species occupying the same geographical area. (wikipedia)

An ecological unit composed of a group of organisms or a population of different species occupying a particular area, usually interacting with each other and their environment. (biology-online.org)</dc:description>
    </owl:Class>
    


    <!-- http://ecoinformatics.org/oboe/oboe.1.0/oboe-ecology.owl#EcologicalHabitat -->

    <owl:Class rdf:about="http://ecoinformatics.org/oboe/oboe.1.0/oboe-ecology.owl#EcologicalHabitat">
        <rdfs:label>Ecological Habitat</rdfs:label>
        <rdfs:subClassOf rdf:resource="&oboe-core;Entity"/>
        <dc:description>Place where an organism or a biological population normally lives or occurs (biololgy-online.org)</dc:description>
    </owl:Class>
    


    <!-- http://ecoinformatics.org/oboe/oboe.1.0/oboe-ecology.owl#Phytoplankton -->

    <owl:Class rdf:about="http://ecoinformatics.org/oboe/oboe.1.0/oboe-ecology.owl#Phytoplankton">
        <rdfs:subClassOf rdf:resource="http://ecoinformatics.org/oboe/oboe.1.0/oboe-ecology.owl#EcologicalCommunity"/>
        <dc:description>Usually microscopic free-floating, photosynthetic organisms in aquatic systems. </dc:description>
    </owl:Class>
    


    <!-- http://ecoinformatics.org/oboe/oboe.1.0/oboe-ecology.owl#Population -->

    <owl:Class rdf:about="http://ecoinformatics.org/oboe/oboe.1.0/oboe-ecology.owl#Population">
        <rdfs:label xml:lang="en">Population</rdfs:label>
        <rdfs:subClassOf rdf:resource="&oboe-core;Entity"/>
        <dc:description xml:lang="en">A set of organisms of the same species within a defined area.</dc:description>
    </owl:Class>
    


    <!-- http://ecoinformatics.org/oboe/oboe.1.0/oboe-ecology.owl#PopulationSample -->

    <owl:Class rdf:about="http://ecoinformatics.org/oboe/oboe.1.0/oboe-ecology.owl#PopulationSample">
        <rdfs:label xml:lang="en">Population Sample</rdfs:label>
        <rdfs:subClassOf rdf:resource="http://ecoinformatics.org/oboe/oboe.1.0/oboe-ecology.owl#Sample"/>
        <dc:description xml:lang="en">A subset of individuals in a biological population.</dc:description>
    </owl:Class>
    


    <!-- http://ecoinformatics.org/oboe/oboe.1.0/oboe-ecology.owl#Sample -->

    <owl:Class rdf:about="http://ecoinformatics.org/oboe/oboe.1.0/oboe-ecology.owl#Sample">
        <rdfs:label xml:lang="en">Sample</rdfs:label>
        <rdfs:subClassOf rdf:resource="&oboe-core;Entity"/>
        <rdfs:comment xml:lang="en">A sample may be material or conceptual in nature,  e.g. tissue sample, rock sample, water sample, statistical population sample, etc.</rdfs:comment>
        <dc:description xml:lang="en">A subset of an entity.</dc:description>
    </owl:Class>
    


    <!-- http://ecoinformatics.org/oboe/oboe.1.0/oboe-ecology.owl#StreamHabitat -->

    <owl:Class rdf:about="http://ecoinformatics.org/oboe/oboe.1.0/oboe-ecology.owl#StreamHabitat">
        <rdfs:label>Stream Habitat</rdfs:label>
        <rdfs:subClassOf rdf:resource="http://ecoinformatics.org/oboe/oboe.1.0/oboe-ecology.owl#EcologicalHabitat"/>
        <rdfs:comment>TO DO MOB: find similarConceptTo</rdfs:comment>
        <rdfs:comment>This habitat should have an object property that ties it to a Stream Environment.</rdfs:comment>
    </owl:Class>
    


    <!-- http://ecoinformatics.org/oboe/oboe.1.0/oboe-ecology.owl#TemperateReefHabitat -->

    <owl:Class rdf:about="http://ecoinformatics.org/oboe/oboe.1.0/oboe-ecology.owl#TemperateReefHabitat">
        <rdfs:label>Temperate Reef Habitat</rdfs:label>
        <rdfs:subClassOf rdf:resource="http://ecoinformatics.org/oboe/oboe.1.0/oboe-ecology.owl#EcologicalHabitat"/>
        <rdfs:comment>This habitat should have an object property that ties it to a Temperate Reef Environment</rdfs:comment>
        <rdfs:comment>TO DO MOB: find similarConceptTo</rdfs:comment>
    </owl:Class>
    


    <!-- http://ecoinformatics.org/oboe/oboe.1.0/oboe-ecology.owl#WaterSample -->

    <owl:Class rdf:about="http://ecoinformatics.org/oboe/oboe.1.0/oboe-ecology.owl#WaterSample">
        <rdfs:label>Water Sample</rdfs:label>
        <rdfs:subClassOf rdf:resource="http://ecoinformatics.org/oboe/oboe.1.0/oboe-ecology.owl#Sample"/>
    </owl:Class>
</rdf:RDF>



<!-- Generated by the OWL API (version 3.2.2.1785) http://owlapi.sourceforge.net -->

