<?xml version="1.0"?>
<rdf:RDF xmlns="http://ecoinformatics.org/oboe/oboe.1.2/oboe-core.owl#"
     xml:base="http://ecoinformatics.org/oboe/oboe.1.2/oboe-core.owl"
     xmlns:cc="http://creativecommons.org/ns#"
     xmlns:rdf="http://www.w3.org/1999/02/22-rdf-syntax-ns#"
     xmlns:owl="http://www.w3.org/2002/07/owl#"
     xmlns:xml="http://www.w3.org/XML/1998/namespace"
     xmlns:oboe-core="http://ecoinformatics.org/oboe/oboe.1.2/oboe-core.owl#"
     xmlns:owl2xml="http://www.w3.org/2006/12/owl2-xml#"
     xmlns:swrlb="http://www.w3.org/2003/11/swrlb#"
     xmlns:swrl="http://www.w3.org/2003/11/swrl#"
     xmlns:xsd="http://www.w3.org/2001/XMLSchema#"
     xmlns:rdfs="http://www.w3.org/2000/01/rdf-schema#">
    <owl:Ontology rdf:about="http://ecoinformatics.org/oboe/oboe.1.2/oboe-core.owl">
        <cc:license rdf:datatype="http://www.w3.org/2001/XMLSchema#anyURI">http://creativecommons.org/licenses/by/3.0/</cc:license>
        <rdfs:label>oboe-core</rdfs:label>
        <rdfs:comment>This ontology provides the core OBOE modeling constructs.</rdfs:comment>
        <owl:versionInfo>Version 1.2</owl:versionInfo>
        <rdfs:comment>Copyright (c) 2006-2016 The Regents of the University of California.  All rights reserved. This work is licensed under the Creative Commons Attribution 3.0 Unported License. To view a copy of this license, visit http://creativecommons.org/licenses/by/3.0/ or send a letter to Creative Commons, 444 Castro Street, Suite 900, Mountain View, California, 94041, USA.</rdfs:comment>
    </owl:Ontology>
    


    <!-- 
    ///////////////////////////////////////////////////////////////////////////////////////
    //
    // Annotation properties
    //
    ///////////////////////////////////////////////////////////////////////////////////////
     -->

    


    <!-- http://ecoinformatics.org/oboe/oboe.1.2/oboe-core.owl#sameConceptAs -->

    <owl:AnnotationProperty rdf:about="http://ecoinformatics.org/oboe/oboe.1.2/oboe-core.owl#sameConceptAs">
        <rdfs:comment>A class annotation property that states that the annotated class is conceptually the same class as (i.e., conceptually equivalent to) the concept identified in the annotation value. If the value of the annotation property denotes an OWL class, then the sameConceptAsClass annotation property should be used instead.</rdfs:comment>
    </owl:AnnotationProperty>
    


    <!-- http://ecoinformatics.org/oboe/oboe.1.2/oboe-core.owl#sameConceptAsClass -->

    <owl:AnnotationProperty rdf:about="http://ecoinformatics.org/oboe/oboe.1.2/oboe-core.owl#sameConceptAsClass">
        <rdfs:comment>A class annotation property that states that the annotated class is conceptually the same class as (i.e., conceptually equivalent to) the referenced class (as given by the value of the annotation property). Note that being conceptually the same can differ from strict class equivalance in that the two classes may have different structural definitions within their specific ontologies, e.g., their superclasses and subclasses in the respective ontologies may differ.</rdfs:comment>
    </owl:AnnotationProperty>
    


    <!-- http://ecoinformatics.org/oboe/oboe.1.2/oboe-core.owl#similarConceptAs -->

    <owl:AnnotationProperty rdf:about="http://ecoinformatics.org/oboe/oboe.1.2/oboe-core.owl#similarConceptAs">
        <rdfs:comment>
        A class annotation property that states that the annotated class is conceptually similar (e.g., overlapping), but not identical to the concept identified by the value of the annotation property. If the value of the annotation property denotes an OWL class, then the similarConceptAsClass annotation property should be used instead.</rdfs:comment>
    </owl:AnnotationProperty>
    


    <!-- http://ecoinformatics.org/oboe/oboe.1.2/oboe-core.owl#similarConceptAsClass -->

    <owl:AnnotationProperty rdf:about="http://ecoinformatics.org/oboe/oboe.1.2/oboe-core.owl#similarConceptAsClass">
        <rdfs:comment>A class annotation property that states that the annotated class is conceptually similar (e.g., overlapping), but not identical to the referenced class (the value of the annotation property).</rdfs:comment>
    </owl:AnnotationProperty>
    


    <!-- 
    ///////////////////////////////////////////////////////////////////////////////////////
    //
    // Datatypes
    //
    ///////////////////////////////////////////////////////////////////////////////////////
     -->

    


    <!-- http://www.w3.org/2001/XMLSchema#anyType -->

    <rdfs:Datatype rdf:about="http://www.w3.org/2001/XMLSchema#anyType"/>
    


    <!-- 
    ///////////////////////////////////////////////////////////////////////////////////////
    //
    // Object Properties
    //
    ///////////////////////////////////////////////////////////////////////////////////////
     -->

    


    <!-- http://ecoinformatics.org/oboe/oboe.1.2/oboe-core.owl#characteristicFor -->

    <owl:ObjectProperty rdf:about="http://ecoinformatics.org/oboe/oboe.1.2/oboe-core.owl#characteristicFor">
        <rdf:type rdf:resource="http://www.w3.org/2002/07/owl#FunctionalProperty"/>
        <rdfs:domain rdf:resource="http://ecoinformatics.org/oboe/oboe.1.2/oboe-core.owl#Characteristic"/>
        <rdfs:range rdf:resource="http://ecoinformatics.org/oboe/oboe.1.2/oboe-core.owl#Entity"/>
        <rdfs:comment>The characteristicFor property gives the entity of the characteristic.</rdfs:comment>
    </owl:ObjectProperty>
    


    <!-- http://ecoinformatics.org/oboe/oboe.1.2/oboe-core.owl#entityRelated -->

    <owl:ObjectProperty rdf:about="http://ecoinformatics.org/oboe/oboe.1.2/oboe-core.owl#entityRelated">
        <rdfs:domain rdf:resource="http://ecoinformatics.org/oboe/oboe.1.2/oboe-core.owl#Observation"/>
        <rdfs:range rdf:resource="http://ecoinformatics.org/oboe/oboe.1.2/oboe-core.owl#Observation"/>
        <rdfs:comment>The entityRelated property asserts that the entity of one observation has an observed relationship to the entity in another observation.</rdfs:comment>
    </owl:ObjectProperty>
    


    <!-- http://ecoinformatics.org/oboe/oboe.1.2/oboe-core.owl#hasBaseQualifier -->

    <owl:ObjectProperty rdf:about="http://ecoinformatics.org/oboe/oboe.1.2/oboe-core.owl#hasBaseQualifier">
        <rdf:type rdf:resource="http://www.w3.org/2002/07/owl#FunctionalProperty"/>
        <rdfs:domain rdf:resource="http://ecoinformatics.org/oboe/oboe.1.2/oboe-core.owl#CompositeCharacteristicQualifier"/>
        <rdfs:range rdf:resource="http://ecoinformatics.org/oboe/oboe.1.2/oboe-core.owl#BaseCharacteristicQualifier"/>
        <rdfs:comment>The hasBaseQualifier together with the hasNextQualfiier property allows qualifier characteristics to be combined and ordered. For example, for an MinimumDailyAverage qualifier, the hasBaseQualifier refers to Minimum and the hasNextQualifier refers to a DailyAverage qualifier, and for a DailyAverage qualifier, the hasBaseQualifier refers to a Daily qualifier and the hasNextQualifier refers to an Average qualifier.</rdfs:comment>
    </owl:ObjectProperty>
    


    <!-- http://ecoinformatics.org/oboe/oboe.1.2/oboe-core.owl#hasContext -->

    <owl:ObjectProperty rdf:about="http://ecoinformatics.org/oboe/oboe.1.2/oboe-core.owl#hasContext">
        <rdf:type rdf:resource="http://www.w3.org/2002/07/owl#TransitiveProperty"/>
        <rdfs:domain rdf:resource="http://ecoinformatics.org/oboe/oboe.1.2/oboe-core.owl#Observation"/>
        <rdfs:range rdf:resource="http://ecoinformatics.org/oboe/oboe.1.2/oboe-core.owl#Observation"/>
        <rdfs:comment rdf:datatype="http://www.w3.org/2001/XMLSchema#string">The hasContext property asserts that one observation serves as the context for another observation.  In a hasContext property the domain is the observation being contextualized and the range is the context. Context defines a semantic relationship between two entities that is a fundamental aspect of the observations, but not necessarily of the entities themselves.  For example, most measurements are accomplished in a spatio-temporal framework that might be valuable context. The assertions made by contextual observations are assumed of the contextualized observations. Context is a transitive relationship.</rdfs:comment>
    </owl:ObjectProperty>
    


    <!-- http://ecoinformatics.org/oboe/oboe.1.2/oboe-core.owl#hasMeasurement -->

    <owl:ObjectProperty rdf:about="http://ecoinformatics.org/oboe/oboe.1.2/oboe-core.owl#hasMeasurement">
        <owl:inverseOf rdf:resource="http://ecoinformatics.org/oboe/oboe.1.2/oboe-core.owl#measurementFor"/>
        <rdf:type rdf:resource="http://www.w3.org/2002/07/owl#InverseFunctionalProperty"/>
        <rdfs:domain rdf:resource="http://ecoinformatics.org/oboe/oboe.1.2/oboe-core.owl#Observation"/>
        <rdfs:range rdf:resource="http://ecoinformatics.org/oboe/oboe.1.2/oboe-core.owl#Measurement"/>
        <rdfs:comment rdf:datatype="http://www.w3.org/2001/XMLSchema#string">The hasMeasurement property gives the measurements of the observed entity.</rdfs:comment>
    </owl:ObjectProperty>
    


    <!-- http://ecoinformatics.org/oboe/oboe.1.2/oboe-core.owl#hasMember -->

    <owl:ObjectProperty rdf:about="http://ecoinformatics.org/oboe/oboe.1.2/oboe-core.owl#hasMember">
        <rdfs:domain rdf:resource="http://ecoinformatics.org/oboe/oboe.1.2/oboe-core.owl#ObservationCollection"/>
        <rdfs:range rdf:resource="http://ecoinformatics.org/oboe/oboe.1.2/oboe-core.owl#Observation"/>
        <rdfs:comment>The hasMember property gives the observations of an observation collection.</rdfs:comment>
    </owl:ObjectProperty>
    


    <!-- http://ecoinformatics.org/oboe/oboe.1.2/oboe-core.owl#hasNextQualifier -->

    <owl:ObjectProperty rdf:about="http://ecoinformatics.org/oboe/oboe.1.2/oboe-core.owl#hasNextQualifier">
        <rdf:type rdf:resource="http://www.w3.org/2002/07/owl#FunctionalProperty"/>
        <rdfs:domain rdf:resource="http://ecoinformatics.org/oboe/oboe.1.2/oboe-core.owl#CompositeCharacteristicQualifier"/>
        <rdfs:range rdf:resource="http://ecoinformatics.org/oboe/oboe.1.2/oboe-core.owl#CharacteristicQualifier"/>
        <rdfs:comment>The hasNexQualifier together with the hasBaseQualfiier property allows qualifier characteristics to be combined and ordered. For example, for an MinimumDailyAverage qualifier, the hasBaseQualifier refers to Minimum and the hasNextQualifier refers to a DailyAverage qualifier, and for a DailyAverage qualifier, the hasBaseQualifier refers to a Daily qualifier and the hasNextQualifier refers to an Average qualifier.</rdfs:comment>
    </owl:ObjectProperty>
    


    <!-- http://ecoinformatics.org/oboe/oboe.1.2/oboe-core.owl#hasObservedRelation -->

    <owl:ObjectProperty rdf:about="http://ecoinformatics.org/oboe/oboe.1.2/oboe-core.owl#hasObservedRelation">
        <rdf:type rdf:resource="http://www.w3.org/2002/07/owl#InverseFunctionalProperty"/>
        <rdfs:domain rdf:resource="http://ecoinformatics.org/oboe/oboe.1.2/oboe-core.owl#Observation"/>
        <rdfs:comment>The hasObservedRelation property gives the observed relation of an observation. The observation entity is the source (head) entity of the corresponding relationship that was observed.</rdfs:comment>
    </owl:ObjectProperty>
    


    <!-- http://ecoinformatics.org/oboe/oboe.1.2/oboe-core.owl#hasQualifier -->

    <owl:ObjectProperty rdf:about="http://ecoinformatics.org/oboe/oboe.1.2/oboe-core.owl#hasQualifier">
        <rdf:type rdf:resource="http://www.w3.org/2002/07/owl#FunctionalProperty"/>
        <rdfs:domain rdf:resource="http://ecoinformatics.org/oboe/oboe.1.2/oboe-core.owl#MeasuredCharacteristic"/>
        <rdfs:range rdf:resource="http://ecoinformatics.org/oboe/oboe.1.2/oboe-core.owl#CharacteristicQualifier"/>
        <rdfs:comment>The hasQualifier property assigns an optional characteristic qualifier to a characteristic. Examples of qualifiers are Average, Minimum, Maximum, Daily, etc.</rdfs:comment>
    </owl:ObjectProperty>
    


    <!-- http://ecoinformatics.org/oboe/oboe.1.2/oboe-core.owl#hasSourceUnit -->

    <owl:ObjectProperty rdf:about="http://ecoinformatics.org/oboe/oboe.1.2/oboe-core.owl#hasSourceUnit">
        <rdf:type rdf:resource="http://www.w3.org/2002/07/owl#FunctionalProperty"/>
        <rdfs:domain rdf:resource="http://ecoinformatics.org/oboe/oboe.1.2/oboe-core.owl#UnitConversion"/>
        <rdfs:range rdf:resource="http://ecoinformatics.org/oboe/oboe.1.2/oboe-core.owl#Unit"/>
        <rdfs:comment>The hasSourceUnit property gives the source unit being converted from within a unit conversion.</rdfs:comment>
    </owl:ObjectProperty>
    


    <!-- http://ecoinformatics.org/oboe/oboe.1.2/oboe-core.owl#hasTargetUnit -->

    <owl:ObjectProperty rdf:about="http://ecoinformatics.org/oboe/oboe.1.2/oboe-core.owl#hasTargetUnit">
        <rdf:type rdf:resource="http://www.w3.org/2002/07/owl#FunctionalProperty"/>
        <rdfs:domain rdf:resource="http://ecoinformatics.org/oboe/oboe.1.2/oboe-core.owl#UnitConversion"/>
        <rdfs:range rdf:resource="http://ecoinformatics.org/oboe/oboe.1.2/oboe-core.owl#Unit"/>
        <rdfs:comment>The hasTargetUnit property gives the target unit being converted to within a unit conversion.</rdfs:comment>
    </owl:ObjectProperty>
    


    <!-- http://ecoinformatics.org/oboe/oboe.1.2/oboe-core.owl#hasUnit -->

    <owl:ObjectProperty rdf:about="http://ecoinformatics.org/oboe/oboe.1.2/oboe-core.owl#hasUnit">
        <rdfs:domain>
            <owl:Class>
                <owl:unionOf rdf:parseType="Collection">
                    <rdf:Description rdf:about="http://ecoinformatics.org/oboe/oboe.1.2/oboe-core.owl#CompositeUnit"/>
                    <rdf:Description rdf:about="http://ecoinformatics.org/oboe/oboe.1.2/oboe-core.owl#DerivedUnit"/>
                    <rdf:Description rdf:about="http://ecoinformatics.org/oboe/oboe.1.2/oboe-core.owl#PrefixedUnit"/>
                </owl:unionOf>
            </owl:Class>
        </rdfs:domain>
        <rdfs:range>
            <owl:Class>
                <owl:unionOf rdf:parseType="Collection">
                    <rdf:Description rdf:about="http://ecoinformatics.org/oboe/oboe.1.2/oboe-core.owl#BaseUnit"/>
                    <rdf:Description rdf:about="http://ecoinformatics.org/oboe/oboe.1.2/oboe-core.owl#DerivedUnit"/>
                    <rdf:Description rdf:about="http://ecoinformatics.org/oboe/oboe.1.2/oboe-core.owl#PrefixedUnit"/>
                </owl:unionOf>
            </owl:Class>
        </rdfs:range>
        <rdfs:comment>The hasUnit property gives the underlying base or derived unit for a derived or composite unit, respectively.</rdfs:comment>
    </owl:ObjectProperty>
    


    <!-- http://ecoinformatics.org/oboe/oboe.1.2/oboe-core.owl#hasValue -->

    <owl:ObjectProperty rdf:about="http://ecoinformatics.org/oboe/oboe.1.2/oboe-core.owl#hasValue">
        <rdf:type rdf:resource="http://www.w3.org/2002/07/owl#FunctionalProperty"/>
        <rdfs:domain rdf:resource="http://ecoinformatics.org/oboe/oboe.1.2/oboe-core.owl#Measurement"/>
        <rdfs:range rdf:resource="http://ecoinformatics.org/oboe/oboe.1.2/oboe-core.owl#MeasuredValue"/>
        <rdfs:comment>The hasValue property gives the value of the measurement.</rdfs:comment>
    </owl:ObjectProperty>
    


    <!-- http://ecoinformatics.org/oboe/oboe.1.2/oboe-core.owl#measurementFor -->

    <owl:ObjectProperty rdf:about="http://ecoinformatics.org/oboe/oboe.1.2/oboe-core.owl#measurementFor">
        <rdf:type rdf:resource="http://www.w3.org/2002/07/owl#FunctionalProperty"/>
        <rdfs:domain rdf:resource="http://ecoinformatics.org/oboe/oboe.1.2/oboe-core.owl#Measurement"/>
        <rdfs:range rdf:resource="http://ecoinformatics.org/oboe/oboe.1.2/oboe-core.owl#Observation"/>
        <rdfs:comment>The measurementFor property gives the observation (observed entitiy) that a measurement is associated with. Each measurement is for exactly one observation. </rdfs:comment>
    </owl:ObjectProperty>
    


    <!-- http://ecoinformatics.org/oboe/oboe.1.2/oboe-core.owl#measuresCharacteristic -->

    <owl:ObjectProperty rdf:about="http://ecoinformatics.org/oboe/oboe.1.2/oboe-core.owl#measuresCharacteristic">
        <rdf:type rdf:resource="http://www.w3.org/2002/07/owl#FunctionalProperty"/>
        <rdfs:domain rdf:resource="http://ecoinformatics.org/oboe/oboe.1.2/oboe-core.owl#MeasurementType"/>
        <rdfs:range rdf:resource="http://ecoinformatics.org/oboe/oboe.1.2/oboe-core.owl#Characteristic"/>
        <rdfs:comment>The measuresCharacteristic property gives the Characteristic that would be measured by a MeasurementType.</rdfs:comment>
    </owl:ObjectProperty>
    


    <!-- http://ecoinformatics.org/oboe/oboe.1.2/oboe-core.owl#measuresEntity -->

    <owl:ObjectProperty rdf:about="http://ecoinformatics.org/oboe/oboe.1.2/oboe-core.owl#measuresEntity">
        <rdf:type rdf:resource="http://www.w3.org/2002/07/owl#FunctionalProperty"/>
        <rdfs:domain rdf:resource="http://ecoinformatics.org/oboe/oboe.1.2/oboe-core.owl#MeasurementType"/>
        <rdfs:range rdf:resource="http://ecoinformatics.org/oboe/oboe.1.2/oboe-core.owl#Entity"/>
        <rdfs:comment>The measuresEntity property gives the Entity that would be measured by a MeasurementType.</rdfs:comment>
    </owl:ObjectProperty>
    


    <!-- http://ecoinformatics.org/oboe/oboe.1.2/oboe-core.owl#measuresUsingProtocol -->

    <owl:ObjectProperty rdf:about="http://ecoinformatics.org/oboe/oboe.1.2/oboe-core.owl#measuresUsingProtocol">
        <rdf:type rdf:resource="http://www.w3.org/2002/07/owl#FunctionalProperty"/>
        <rdfs:domain rdf:resource="http://ecoinformatics.org/oboe/oboe.1.2/oboe-core.owl#MeasurementType"/>
        <rdfs:range rdf:resource="http://ecoinformatics.org/oboe/oboe.1.2/oboe-core.owl#Protocol"/>
        <rdfs:comment>The measuresUsingProtocol property gives the Protocol that would be used by a MeasurementType.</rdfs:comment>
    </owl:ObjectProperty>
    


    <!-- http://ecoinformatics.org/oboe/oboe.1.2/oboe-core.owl#measuresUsingStandard -->

    <owl:ObjectProperty rdf:about="http://ecoinformatics.org/oboe/oboe.1.2/oboe-core.owl#measuresUsingStandard">
        <rdf:type rdf:resource="http://www.w3.org/2002/07/owl#FunctionalProperty"/>
        <rdfs:domain rdf:resource="http://ecoinformatics.org/oboe/oboe.1.2/oboe-core.owl#MeasurementType"/>
        <rdfs:range rdf:resource="http://ecoinformatics.org/oboe/oboe.1.2/oboe-core.owl#Standard"/>
        <rdfs:comment>The measuresUsingStandard property gives the Standard that would be used by a MeasurementType.</rdfs:comment>
    </owl:ObjectProperty>
    


    <!-- http://ecoinformatics.org/oboe/oboe.1.2/oboe-core.owl#ofCharacteristic -->

    <owl:ObjectProperty rdf:about="http://ecoinformatics.org/oboe/oboe.1.2/oboe-core.owl#ofCharacteristic">
        <rdf:type rdf:resource="http://www.w3.org/2002/07/owl#FunctionalProperty"/>
        <rdfs:domain rdf:resource="http://ecoinformatics.org/oboe/oboe.1.2/oboe-core.owl#Measurement"/>
        <rdfs:range rdf:resource="http://ecoinformatics.org/oboe/oboe.1.2/oboe-core.owl#Characteristic"/>
        <rdfs:comment>The ofCharacteristic property gives the entity characteristic measured by a measurement.</rdfs:comment>
    </owl:ObjectProperty>
    


    <!-- http://ecoinformatics.org/oboe/oboe.1.2/oboe-core.owl#ofEntity -->

    <owl:ObjectProperty rdf:about="http://ecoinformatics.org/oboe/oboe.1.2/oboe-core.owl#ofEntity">
        <rdf:type rdf:resource="http://www.w3.org/2002/07/owl#FunctionalProperty"/>
        <rdfs:domain rdf:resource="http://ecoinformatics.org/oboe/oboe.1.2/oboe-core.owl#Observation"/>
        <rdfs:range rdf:resource="http://ecoinformatics.org/oboe/oboe.1.2/oboe-core.owl#Entity"/>
        <rdfs:comment rdf:datatype="http://www.w3.org/2001/XMLSchema#string">The ofEntity property gives the observed entity of an observation.</rdfs:comment>
    </owl:ObjectProperty>
    


    <!-- http://ecoinformatics.org/oboe/oboe.1.2/oboe-core.owl#usesProtocol -->

    <owl:ObjectProperty rdf:about="http://ecoinformatics.org/oboe/oboe.1.2/oboe-core.owl#usesProtocol">
        <rdf:type rdf:resource="http://www.w3.org/2002/07/owl#FunctionalProperty"/>
        <rdf:type rdf:resource="http://www.w3.org/2002/07/owl#InverseFunctionalProperty"/>
        <rdfs:domain rdf:resource="http://ecoinformatics.org/oboe/oboe.1.2/oboe-core.owl#Measurement"/>
        <rdfs:range rdf:resource="http://ecoinformatics.org/oboe/oboe.1.2/oboe-core.owl#Protocol"/>
        <rdfs:comment>The usesProtocol property gives the protocol used in a measurement.</rdfs:comment>
    </owl:ObjectProperty>
    


    <!-- http://ecoinformatics.org/oboe/oboe.1.2/oboe-core.owl#usesStandard -->

    <owl:ObjectProperty rdf:about="http://ecoinformatics.org/oboe/oboe.1.2/oboe-core.owl#usesStandard">
        <rdf:type rdf:resource="http://www.w3.org/2002/07/owl#FunctionalProperty"/>
        <rdf:type rdf:resource="http://www.w3.org/2002/07/owl#InverseFunctionalProperty"/>
        <rdfs:domain rdf:resource="http://ecoinformatics.org/oboe/oboe.1.2/oboe-core.owl#Measurement"/>
        <rdfs:range rdf:resource="http://ecoinformatics.org/oboe/oboe.1.2/oboe-core.owl#Standard"/>
        <rdfs:comment rdf:datatype="http://www.w3.org/2001/XMLSchema#string">The usesStandard property gives the standard (e.g., unit) used in a measurement.</rdfs:comment>
    </owl:ObjectProperty>
    


    <!-- 
    ///////////////////////////////////////////////////////////////////////////////////////
    //
    // Data properties
    //
    ///////////////////////////////////////////////////////////////////////////////////////
     -->

    


    <!-- http://ecoinformatics.org/oboe/oboe.1.2/oboe-core.owl#hasCode -->

    <owl:DatatypeProperty rdf:about="http://ecoinformatics.org/oboe/oboe.1.2/oboe-core.owl#hasCode">
        <rdf:type rdf:resource="http://www.w3.org/2002/07/owl#FunctionalProperty"/>
        <rdfs:domain rdf:resource="http://ecoinformatics.org/oboe/oboe.1.2/oboe-core.owl#MeasuredValue"/>
        <rdfs:comment>The hasCode property gives the underlying value (or coded representation) of a primitive value.</rdfs:comment>
    </owl:DatatypeProperty>
    


    <!-- http://ecoinformatics.org/oboe/oboe.1.2/oboe-core.owl#hasMultiplier -->

    <owl:DatatypeProperty rdf:about="http://ecoinformatics.org/oboe/oboe.1.2/oboe-core.owl#hasMultiplier">
        <rdf:type rdf:resource="http://www.w3.org/2002/07/owl#FunctionalProperty"/>
        <rdfs:domain rdf:resource="http://ecoinformatics.org/oboe/oboe.1.2/oboe-core.owl#UnitConversion"/>
        <rdfs:range rdf:resource="http://www.w3.org/2001/XMLSchema#decimal"/>
        <rdfs:comment>The hasMultiplier property gives the multiplier value in a unit conversion.</rdfs:comment>
    </owl:DatatypeProperty>
    


    <!-- http://ecoinformatics.org/oboe/oboe.1.2/oboe-core.owl#hasOffset -->

    <owl:DatatypeProperty rdf:about="http://ecoinformatics.org/oboe/oboe.1.2/oboe-core.owl#hasOffset">
        <rdf:type rdf:resource="http://www.w3.org/2002/07/owl#FunctionalProperty"/>
        <rdfs:domain rdf:resource="http://ecoinformatics.org/oboe/oboe.1.2/oboe-core.owl#UnitConversion"/>
        <rdfs:range rdf:resource="http://www.w3.org/2001/XMLSchema#decimal"/>
        <rdfs:comment>The hasOffset property gives the offset value in a unit conversion.</rdfs:comment>
    </owl:DatatypeProperty>
    


    <!-- http://ecoinformatics.org/oboe/oboe.1.2/oboe-core.owl#hasPower -->

    <owl:DatatypeProperty rdf:about="http://ecoinformatics.org/oboe/oboe.1.2/oboe-core.owl#hasPower">
        <rdf:type rdf:resource="http://www.w3.org/2002/07/owl#FunctionalProperty"/>
        <rdfs:domain rdf:resource="http://ecoinformatics.org/oboe/oboe.1.2/oboe-core.owl#DerivedUnit"/>
        <rdfs:range rdf:resource="http://www.w3.org/2001/XMLSchema#int"/>
        <rdfs:comment>The hasPower property gives the power a base unit is raised to within a derived unit.</rdfs:comment>
    </owl:DatatypeProperty>
    


    <!-- http://ecoinformatics.org/oboe/oboe.1.2/oboe-core.owl#hasPrecision -->

    <owl:DatatypeProperty rdf:about="http://ecoinformatics.org/oboe/oboe.1.2/oboe-core.owl#hasPrecision">
        <rdf:type rdf:resource="http://www.w3.org/2002/07/owl#FunctionalProperty"/>
        <rdfs:domain rdf:resource="http://ecoinformatics.org/oboe/oboe.1.2/oboe-core.owl#Measurement"/>
        <rdfs:range rdf:resource="http://www.w3.org/2001/XMLSchema#decimal"/>
        <rdfs:comment rdf:datatype="http://www.w3.org/2001/XMLSchema#string">This property gives the precision of a measurement value.</rdfs:comment>
    </owl:DatatypeProperty>
    


    <!-- http://ecoinformatics.org/oboe/oboe.1.2/oboe-core.owl#hasPrefixMultiplier -->

    <owl:DatatypeProperty rdf:about="http://ecoinformatics.org/oboe/oboe.1.2/oboe-core.owl#hasPrefixMultiplier">
        <rdf:type rdf:resource="http://www.w3.org/2002/07/owl#FunctionalProperty"/>
        <rdfs:domain rdf:resource="http://ecoinformatics.org/oboe/oboe.1.2/oboe-core.owl#PrefixedUnit"/>
        <rdfs:range rdf:resource="http://www.w3.org/2001/XMLSchema#decimal"/>
    </owl:DatatypeProperty>
    


    <!-- http://ecoinformatics.org/oboe/oboe.1.2/oboe-core.owl#usesMethod -->

    <owl:DatatypeProperty rdf:about="http://ecoinformatics.org/oboe/oboe.1.2/oboe-core.owl#usesMethod">
        <rdf:type rdf:resource="http://www.w3.org/2002/07/owl#FunctionalProperty"/>
        <rdfs:domain rdf:resource="http://ecoinformatics.org/oboe/oboe.1.2/oboe-core.owl#Measurement"/>
        <rdfs:comment>The usesMethod property gives the actual method used to carry out the measurement.</rdfs:comment>
    </owl:DatatypeProperty>
    


    <!-- 
    ///////////////////////////////////////////////////////////////////////////////////////
    //
    // Classes
    //
    ///////////////////////////////////////////////////////////////////////////////////////
     -->

    


    <!-- http://ecoinformatics.org/oboe/oboe.1.2/oboe-core.owl#BaseCharacteristicQualifier -->

    <owl:Class rdf:about="http://ecoinformatics.org/oboe/oboe.1.2/oboe-core.owl#BaseCharacteristicQualifier">
        <rdfs:subClassOf rdf:resource="http://ecoinformatics.org/oboe/oboe.1.2/oboe-core.owl#CharacteristicQualifier"/>
        <rdfs:comment>A base qualifier denotes a simple, atomic qualifier such as average, minimum, and maximum.</rdfs:comment>
        <rdfs:label xml:lang="en">Base Characteristic Qualifier</rdfs:label>
    </owl:Class>
    


    <!-- http://ecoinformatics.org/oboe/oboe.1.2/oboe-core.owl#BaseUnit -->

    <owl:Class rdf:about="http://ecoinformatics.org/oboe/oboe.1.2/oboe-core.owl#BaseUnit">
        <rdfs:subClassOf rdf:resource="http://ecoinformatics.org/oboe/oboe.1.2/oboe-core.owl#Unit"/>
        <owl:disjointWith rdf:resource="http://ecoinformatics.org/oboe/oboe.1.2/oboe-core.owl#CompositeUnit"/>
        <owl:disjointWith rdf:resource="http://ecoinformatics.org/oboe/oboe.1.2/oboe-core.owl#DerivedUnit"/>
        <owl:disjointWith rdf:resource="http://ecoinformatics.org/oboe/oboe.1.2/oboe-core.owl#PrefixedUnit"/>
        <rdfs:comment>A base unit is a unit that is not naturally decomposed into other units.</rdfs:comment>
        <rdfs:label xml:lang="en">Base Unit</rdfs:label>
    </owl:Class>
    


    <!-- http://ecoinformatics.org/oboe/oboe.1.2/oboe-core.owl#CategoricalStandard -->

    <owl:Class rdf:about="http://ecoinformatics.org/oboe/oboe.1.2/oboe-core.owl#CategoricalStandard">
        <rdfs:subClassOf rdf:resource="http://ecoinformatics.org/oboe/oboe.1.2/oboe-core.owl#Standard"/>
        <owl:disjointWith rdf:resource="http://ecoinformatics.org/oboe/oboe.1.2/oboe-core.owl#Index"/>
        <owl:disjointWith rdf:resource="http://ecoinformatics.org/oboe/oboe.1.2/oboe-core.owl#Unit"/>
    </owl:Class>
    


    <!-- http://ecoinformatics.org/oboe/oboe.1.2/oboe-core.owl#Characteristic -->

    <owl:Class rdf:about="http://ecoinformatics.org/oboe/oboe.1.2/oboe-core.owl#Characteristic">
        <rdfs:subClassOf>
            <owl:Restriction>
                <owl:onProperty rdf:resource="http://ecoinformatics.org/oboe/oboe.1.2/oboe-core.owl#characteristicFor"/>
                <owl:someValuesFrom rdf:resource="http://ecoinformatics.org/oboe/oboe.1.2/oboe-core.owl#Entity"/>
            </owl:Restriction>
        </rdfs:subClassOf>
        <owl:disjointWith rdf:resource="http://ecoinformatics.org/oboe/oboe.1.2/oboe-core.owl#CharacteristicQualifier"/>
        <owl:disjointWith rdf:resource="http://ecoinformatics.org/oboe/oboe.1.2/oboe-core.owl#Entity"/>
        <owl:disjointWith rdf:resource="http://ecoinformatics.org/oboe/oboe.1.2/oboe-core.owl#MeasuredValue"/>
        <owl:disjointWith rdf:resource="http://ecoinformatics.org/oboe/oboe.1.2/oboe-core.owl#Measurement"/>
        <owl:disjointWith rdf:resource="http://ecoinformatics.org/oboe/oboe.1.2/oboe-core.owl#MeasurementType"/>
        <owl:disjointWith rdf:resource="http://ecoinformatics.org/oboe/oboe.1.2/oboe-core.owl#Observation"/>
        <owl:disjointWith rdf:resource="http://ecoinformatics.org/oboe/oboe.1.2/oboe-core.owl#ObservationCollection"/>
        <owl:disjointWith rdf:resource="http://ecoinformatics.org/oboe/oboe.1.2/oboe-core.owl#Protocol"/>
        <owl:disjointWith rdf:resource="http://ecoinformatics.org/oboe/oboe.1.2/oboe-core.owl#Standard"/>
        <rdfs:comment rdf:datatype="http://www.w3.org/2001/XMLSchema#string">A characteristic represents a property of an entity that can be measured (e.g., height, length, or color).  A characteristic of an entity is observed through a measurement, which further asserts a value of the characteristic for the entity. A characteristic type (e.g., &quot;height&quot;) can be associated with many different entities, whereas an individual characteristic (a particular occurrence of the &quot;height&quot; characteristic) is associated to exactly one entity.</rdfs:comment>
        <rdfs:label xml:lang="en">Characteristic</rdfs:label>
    </owl:Class>
    


    <!-- http://ecoinformatics.org/oboe/oboe.1.2/oboe-core.owl#CharacteristicQualifier -->

    <owl:Class rdf:about="http://ecoinformatics.org/oboe/oboe.1.2/oboe-core.owl#CharacteristicQualifier">
        <owl:equivalentClass>
            <owl:Class>
                <owl:unionOf rdf:parseType="Collection">
                    <rdf:Description rdf:about="http://ecoinformatics.org/oboe/oboe.1.2/oboe-core.owl#BaseCharacteristicQualifier"/>
                    <rdf:Description rdf:about="http://ecoinformatics.org/oboe/oboe.1.2/oboe-core.owl#CompositeCharacteristicQualifier"/>
                </owl:unionOf>
            </owl:Class>
        </owl:equivalentClass>
        <owl:disjointWith rdf:resource="http://ecoinformatics.org/oboe/oboe.1.2/oboe-core.owl#Entity"/>
        <owl:disjointWith rdf:resource="http://ecoinformatics.org/oboe/oboe.1.2/oboe-core.owl#MeasuredValue"/>
        <owl:disjointWith rdf:resource="http://ecoinformatics.org/oboe/oboe.1.2/oboe-core.owl#Measurement"/>
        <owl:disjointWith rdf:resource="http://ecoinformatics.org/oboe/oboe.1.2/oboe-core.owl#MeasurementType"/>
        <owl:disjointWith rdf:resource="http://ecoinformatics.org/oboe/oboe.1.2/oboe-core.owl#Observation"/>
        <owl:disjointWith rdf:resource="http://ecoinformatics.org/oboe/oboe.1.2/oboe-core.owl#ObservationCollection"/>
        <owl:disjointWith rdf:resource="http://ecoinformatics.org/oboe/oboe.1.2/oboe-core.owl#Protocol"/>
        <owl:disjointWith rdf:resource="http://ecoinformatics.org/oboe/oboe.1.2/oboe-core.owl#Standard"/>
        <owl:disjointWith rdf:resource="http://ecoinformatics.org/oboe/oboe.1.2/oboe-core.owl#UnitConversion"/>
        <rdfs:comment>A characteristic qualifier is a derived property of an entity that must be combined with concrete characteristics to be used in a measurement. A qualifier is either a base (atomic) or composite qualifier. As an example, the base qualifier minimum can be combined with a characteristic length to create a minimum length qualified characteristic. A composite qualifer is used to combine multiple qualifiers.</rdfs:comment>
        <rdfs:label xml:lang="en">Characteristic Qualifier</rdfs:label>
    </owl:Class>
    


    <!-- http://ecoinformatics.org/oboe/oboe.1.2/oboe-core.owl#CompositeCharacteristicQualifier -->

    <owl:Class rdf:about="http://ecoinformatics.org/oboe/oboe.1.2/oboe-core.owl#CompositeCharacteristicQualifier">
        <rdfs:subClassOf rdf:resource="http://ecoinformatics.org/oboe/oboe.1.2/oboe-core.owl#CharacteristicQualifier"/>
        <rdfs:subClassOf>
            <owl:Restriction>
                <owl:onProperty rdf:resource="http://ecoinformatics.org/oboe/oboe.1.2/oboe-core.owl#hasBaseQualifier"/>
                <owl:qualifiedCardinality rdf:datatype="http://www.w3.org/2001/XMLSchema#nonNegativeInteger">1</owl:qualifiedCardinality>
                <owl:onClass rdf:resource="http://ecoinformatics.org/oboe/oboe.1.2/oboe-core.owl#BaseCharacteristicQualifier"/>
            </owl:Restriction>
        </rdfs:subClassOf>
        <rdfs:subClassOf>
            <owl:Restriction>
                <owl:onProperty rdf:resource="http://ecoinformatics.org/oboe/oboe.1.2/oboe-core.owl#hasNextQualifier"/>
                <owl:qualifiedCardinality rdf:datatype="http://www.w3.org/2001/XMLSchema#nonNegativeInteger">1</owl:qualifiedCardinality>
                <owl:onClass rdf:resource="http://ecoinformatics.org/oboe/oboe.1.2/oboe-core.owl#CharacteristicQualifier"/>
            </owl:Restriction>
        </rdfs:subClassOf>
        <rdfs:comment>A composite qualifier combines multiple qualifiers. Each composite qualifier has a base qualifier and a reference to another qualifier. Composite qualifiers are ordered (through hasNextQualifier) to distinguish between the scope of qualifiers, e.g., AverageMinimum versus MinimumAverage.</rdfs:comment>
        <rdfs:label xml:lang="en">Composite Characteristic Qualifier</rdfs:label>
    </owl:Class>
    


    <!-- http://ecoinformatics.org/oboe/oboe.1.2/oboe-core.owl#CompositeUnit -->

    <owl:Class rdf:about="http://ecoinformatics.org/oboe/oboe.1.2/oboe-core.owl#CompositeUnit">
        <rdfs:subClassOf rdf:resource="http://ecoinformatics.org/oboe/oboe.1.2/oboe-core.owl#Unit"/>
        <rdfs:subClassOf>
            <owl:Restriction>
                <owl:onProperty rdf:resource="http://ecoinformatics.org/oboe/oboe.1.2/oboe-core.owl#hasUnit"/>
                <owl:minQualifiedCardinality rdf:datatype="http://www.w3.org/2001/XMLSchema#nonNegativeInteger">2</owl:minQualifiedCardinality>
                <owl:onClass>
                    <owl:Class>
                        <owl:unionOf rdf:parseType="Collection">
                            <rdf:Description rdf:about="http://ecoinformatics.org/oboe/oboe.1.2/oboe-core.owl#BaseUnit"/>
                            <rdf:Description rdf:about="http://ecoinformatics.org/oboe/oboe.1.2/oboe-core.owl#DerivedUnit"/>
                            <rdf:Description rdf:about="http://ecoinformatics.org/oboe/oboe.1.2/oboe-core.owl#PrefixedUnit"/>
                        </owl:unionOf>
                    </owl:Class>
                </owl:onClass>
            </owl:Restriction>
        </rdfs:subClassOf>
        <owl:disjointWith rdf:resource="http://ecoinformatics.org/oboe/oboe.1.2/oboe-core.owl#DerivedUnit"/>
        <owl:disjointWith rdf:resource="http://ecoinformatics.org/oboe/oboe.1.2/oboe-core.owl#PrefixedUnit"/>
        <rdfs:comment>A composite unit is the product of at least two base or derived units. For example, &apos;meter per second square&apos; denotes a composite unit defined over &apos;meter&apos; (a base unit) and &apos;per second square&apos; (a derived unit).</rdfs:comment>
        <rdfs:label xml:lang="en">Composite Unit</rdfs:label>
    </owl:Class>
    


    <!-- http://ecoinformatics.org/oboe/oboe.1.2/oboe-core.owl#DerivedUnit -->

    <owl:Class rdf:about="http://ecoinformatics.org/oboe/oboe.1.2/oboe-core.owl#DerivedUnit">
        <rdfs:subClassOf rdf:resource="http://ecoinformatics.org/oboe/oboe.1.2/oboe-core.owl#Unit"/>
        <rdfs:subClassOf>
            <owl:Class>
                <owl:complementOf>
                    <owl:Restriction>
                        <owl:onProperty rdf:resource="http://ecoinformatics.org/oboe/oboe.1.2/oboe-core.owl#hasPower"/>
                        <owl:hasValue rdf:datatype="http://www.w3.org/2001/XMLSchema#integer">0</owl:hasValue>
                    </owl:Restriction>
                </owl:complementOf>
            </owl:Class>
        </rdfs:subClassOf>
        <rdfs:subClassOf>
            <owl:Class>
                <owl:complementOf>
                    <owl:Restriction>
                        <owl:onProperty rdf:resource="http://ecoinformatics.org/oboe/oboe.1.2/oboe-core.owl#hasPower"/>
                        <owl:hasValue rdf:datatype="http://www.w3.org/2001/XMLSchema#integer">1</owl:hasValue>
                    </owl:Restriction>
                </owl:complementOf>
            </owl:Class>
        </rdfs:subClassOf>
        <rdfs:subClassOf>
            <owl:Restriction>
                <owl:onProperty rdf:resource="http://ecoinformatics.org/oboe/oboe.1.2/oboe-core.owl#hasPower"/>
                <owl:someValuesFrom rdf:resource="http://www.w3.org/2001/XMLSchema#int"/>
            </owl:Restriction>
        </rdfs:subClassOf>
        <owl:disjointWith rdf:resource="http://ecoinformatics.org/oboe/oboe.1.2/oboe-core.owl#PrefixedUnit"/>
        <rdfs:comment>A derived unit raises a base or prefixed unit to an integer power other than 0 or 1. For example, the unit &apos;square meter&apos; is a unit derived from the &apos;meter&apos; base unit raised to the power 2. As another example, a &apos;square centimeter&apos; is a unit derived from the &apos;centimeter&apos; prefixed unit raised to the power 2.

BRL 20160601: I removed this restriction so that CompositeUnits like XXXPerLiter would not reason to owl:Nothing. hasUnit exactly 1 (BaseUnit or PrefixedUnit)</rdfs:comment>
        <rdfs:label xml:lang="en">Derived Unit</rdfs:label>
    </owl:Class>
    


    <!-- http://ecoinformatics.org/oboe/oboe.1.2/oboe-core.owl#Entity -->

    <owl:Class rdf:about="http://ecoinformatics.org/oboe/oboe.1.2/oboe-core.owl#Entity">
        <owl:disjointWith rdf:resource="http://ecoinformatics.org/oboe/oboe.1.2/oboe-core.owl#Measurement"/>
        <owl:disjointWith rdf:resource="http://ecoinformatics.org/oboe/oboe.1.2/oboe-core.owl#MeasurementType"/>
        <owl:disjointWith rdf:resource="http://ecoinformatics.org/oboe/oboe.1.2/oboe-core.owl#Observation"/>
        <owl:disjointWith rdf:resource="http://ecoinformatics.org/oboe/oboe.1.2/oboe-core.owl#ObservationCollection"/>
        <owl:disjointWith rdf:resource="http://ecoinformatics.org/oboe/oboe.1.2/oboe-core.owl#Protocol"/>
        <owl:disjointWith rdf:resource="http://ecoinformatics.org/oboe/oboe.1.2/oboe-core.owl#Standard"/>
        <rdfs:comment rdf:datatype="http://www.w3.org/2001/XMLSchema#string">An entity is an object (e.g., a tree, a community, an ecological process). Entities constitute the foci of observations, i.e., every observation is of exactly one entity.</rdfs:comment>
        <rdfs:label xml:lang="en">Entity</rdfs:label>
    </owl:Class>
    


    <!-- http://ecoinformatics.org/oboe/oboe.1.2/oboe-core.owl#IdentifyingCharacteristic -->

    <owl:Class rdf:about="http://ecoinformatics.org/oboe/oboe.1.2/oboe-core.owl#IdentifyingCharacteristic">
        <rdfs:subClassOf rdf:resource="http://ecoinformatics.org/oboe/oboe.1.2/oboe-core.owl#Characteristic"/>
        <owl:disjointWith rdf:resource="http://ecoinformatics.org/oboe/oboe.1.2/oboe-core.owl#MeasuredCharacteristic"/>
        <rdfs:comment>An identifying characteristic is used to identify or name an entity either globally or within a context, such as a name of a lake or a tag number assigned to a tree. Unlike a MeasuredCharacteristic, an IdentifyingCharacteristic is assigned and not measured.</rdfs:comment>
        <rdfs:label xml:lang="en">Identifying Characteristic</rdfs:label>
    </owl:Class>
    


    <!-- http://ecoinformatics.org/oboe/oboe.1.2/oboe-core.owl#Index -->

    <owl:Class rdf:about="http://ecoinformatics.org/oboe/oboe.1.2/oboe-core.owl#Index">
        <rdfs:subClassOf rdf:resource="http://ecoinformatics.org/oboe/oboe.1.2/oboe-core.owl#Standard"/>
        <owl:disjointWith rdf:resource="http://ecoinformatics.org/oboe/oboe.1.2/oboe-core.owl#Unit"/>
    </owl:Class>
    


    <!-- http://ecoinformatics.org/oboe/oboe.1.2/oboe-core.owl#MeasuredCharacteristic -->

    <owl:Class rdf:about="http://ecoinformatics.org/oboe/oboe.1.2/oboe-core.owl#MeasuredCharacteristic">
        <rdfs:subClassOf rdf:resource="http://ecoinformatics.org/oboe/oboe.1.2/oboe-core.owl#Characteristic"/>
        <rdfs:comment>A measured characteristic of an entity is one that is measurable within the physical world. A measured characteristic includes primary and derived physical dimensions (e.g., length, mass, area, density). The measured value assigned to a measured characteristic may be a quantity (a numerical value) or a quality (a category), including both nominal and ordinal categories.</rdfs:comment>
        <rdfs:label xml:lang="en">Measured Characteristic</rdfs:label>
    </owl:Class>
    


    <!-- http://ecoinformatics.org/oboe/oboe.1.2/oboe-core.owl#MeasuredValue -->

    <owl:Class rdf:about="http://ecoinformatics.org/oboe/oboe.1.2/oboe-core.owl#MeasuredValue">
        <owl:disjointWith rdf:resource="http://ecoinformatics.org/oboe/oboe.1.2/oboe-core.owl#Measurement"/>
        <owl:disjointWith rdf:resource="http://ecoinformatics.org/oboe/oboe.1.2/oboe-core.owl#MeasurementType"/>
        <owl:disjointWith rdf:resource="http://ecoinformatics.org/oboe/oboe.1.2/oboe-core.owl#Observation"/>
        <owl:disjointWith rdf:resource="http://ecoinformatics.org/oboe/oboe.1.2/oboe-core.owl#ObservationCollection"/>
        <owl:disjointWith rdf:resource="http://ecoinformatics.org/oboe/oboe.1.2/oboe-core.owl#Protocol"/>
        <owl:disjointWith rdf:resource="http://ecoinformatics.org/oboe/oboe.1.2/oboe-core.owl#Standard"/>
        <owl:disjointWith rdf:resource="http://ecoinformatics.org/oboe/oboe.1.2/oboe-core.owl#UnitConversion"/>
        <rdfs:comment>A measurement value is a quantitative or qualitative result of a measurement. Measurement values can contain a coded representation of the result, e.g., as a number or string.</rdfs:comment>
        <rdfs:label xml:lang="en">Measurement Value</rdfs:label>
    </owl:Class>
    


    <!-- http://ecoinformatics.org/oboe/oboe.1.2/oboe-core.owl#Measurement -->

    <owl:Class rdf:about="http://ecoinformatics.org/oboe/oboe.1.2/oboe-core.owl#Measurement">
        <rdfs:subClassOf>
            <owl:Restriction>
                <owl:onProperty rdf:resource="http://ecoinformatics.org/oboe/oboe.1.2/oboe-core.owl#hasValue"/>
                <owl:someValuesFrom rdf:resource="http://ecoinformatics.org/oboe/oboe.1.2/oboe-core.owl#MeasuredValue"/>
            </owl:Restriction>
        </rdfs:subClassOf>
        <rdfs:subClassOf>
            <owl:Restriction>
                <owl:onProperty rdf:resource="http://ecoinformatics.org/oboe/oboe.1.2/oboe-core.owl#ofCharacteristic"/>
                <owl:someValuesFrom rdf:resource="http://ecoinformatics.org/oboe/oboe.1.2/oboe-core.owl#Characteristic"/>
            </owl:Restriction>
        </rdfs:subClassOf>
        <rdfs:subClassOf>
            <owl:Restriction>
                <owl:onProperty rdf:resource="http://ecoinformatics.org/oboe/oboe.1.2/oboe-core.owl#usesProtocol"/>
                <owl:someValuesFrom rdf:resource="http://ecoinformatics.org/oboe/oboe.1.2/oboe-core.owl#Protocol"/>
            </owl:Restriction>
        </rdfs:subClassOf>
        <rdfs:subClassOf>
            <owl:Restriction>
                <owl:onProperty rdf:resource="http://ecoinformatics.org/oboe/oboe.1.2/oboe-core.owl#usesStandard"/>
                <owl:someValuesFrom rdf:resource="http://ecoinformatics.org/oboe/oboe.1.2/oboe-core.owl#Standard"/>
            </owl:Restriction>
        </rdfs:subClassOf>
        <rdfs:subClassOf>
            <owl:Restriction>
                <owl:onProperty rdf:resource="http://ecoinformatics.org/oboe/oboe.1.2/oboe-core.owl#measurementFor"/>
                <owl:qualifiedCardinality rdf:datatype="http://www.w3.org/2001/XMLSchema#nonNegativeInteger">1</owl:qualifiedCardinality>
                <owl:onClass rdf:resource="http://ecoinformatics.org/oboe/oboe.1.2/oboe-core.owl#Observation"/>
            </owl:Restriction>
        </rdfs:subClassOf>
        <owl:disjointWith rdf:resource="http://ecoinformatics.org/oboe/oboe.1.2/oboe-core.owl#MeasurementType"/>
        <owl:disjointWith rdf:resource="http://ecoinformatics.org/oboe/oboe.1.2/oboe-core.owl#Observation"/>
        <owl:disjointWith rdf:resource="http://ecoinformatics.org/oboe/oboe.1.2/oboe-core.owl#ObservationCollection"/>
        <owl:disjointWith rdf:resource="http://ecoinformatics.org/oboe/oboe.1.2/oboe-core.owl#Protocol"/>
        <owl:disjointWith rdf:resource="http://ecoinformatics.org/oboe/oboe.1.2/oboe-core.owl#Standard"/>
        <rdfs:comment rdf:datatype="http://www.w3.org/2001/XMLSchema#string">A measurement is an assertion that a characteristic of an entity had a particular value with respect to an observation event.  A measurement is comprised of a characteristic, a value, a measurement standard, and a protocol. Measurements can also have precision as well as a description of the methods used. Measurements can encapsulate characteristics that were recorded, but not necessarily measured in a physical sense.  For example, the name of a location and a taxon can be captured through measurements.</rdfs:comment>
        <rdfs:label xml:lang="en">Measurement</rdfs:label>
    </owl:Class>
    


    <!-- http://ecoinformatics.org/oboe/oboe.1.2/oboe-core.owl#MeasurementType -->

    <owl:Class rdf:about="http://ecoinformatics.org/oboe/oboe.1.2/oboe-core.owl#MeasurementType">
        <rdfs:subClassOf>
            <owl:Restriction>
                <owl:onProperty rdf:resource="http://ecoinformatics.org/oboe/oboe.1.2/oboe-core.owl#measuresCharacteristic"/>
                <owl:someValuesFrom rdf:resource="http://ecoinformatics.org/oboe/oboe.1.2/oboe-core.owl#Characteristic"/>
            </owl:Restriction>
        </rdfs:subClassOf>
        <rdfs:subClassOf>
            <owl:Restriction>
                <owl:onProperty rdf:resource="http://ecoinformatics.org/oboe/oboe.1.2/oboe-core.owl#measuresEntity"/>
                <owl:someValuesFrom rdf:resource="http://ecoinformatics.org/oboe/oboe.1.2/oboe-core.owl#Entity"/>
            </owl:Restriction>
        </rdfs:subClassOf>
        <rdfs:subClassOf>
            <owl:Restriction>
                <owl:onProperty rdf:resource="http://ecoinformatics.org/oboe/oboe.1.2/oboe-core.owl#measuresUsingProtocol"/>
                <owl:someValuesFrom rdf:resource="http://ecoinformatics.org/oboe/oboe.1.2/oboe-core.owl#Protocol"/>
            </owl:Restriction>
        </rdfs:subClassOf>
        <rdfs:subClassOf>
            <owl:Restriction>
                <owl:onProperty rdf:resource="http://ecoinformatics.org/oboe/oboe.1.2/oboe-core.owl#measuresUsingStandard"/>
                <owl:someValuesFrom rdf:resource="http://ecoinformatics.org/oboe/oboe.1.2/oboe-core.owl#Standard"/>
            </owl:Restriction>
        </rdfs:subClassOf>
        <owl:disjointWith rdf:resource="http://ecoinformatics.org/oboe/oboe.1.2/oboe-core.owl#Observation"/>
        <owl:disjointWith rdf:resource="http://ecoinformatics.org/oboe/oboe.1.2/oboe-core.owl#ObservationCollection"/>
        <owl:disjointWith rdf:resource="http://ecoinformatics.org/oboe/oboe.1.2/oboe-core.owl#Protocol"/>
        <owl:disjointWith rdf:resource="http://ecoinformatics.org/oboe/oboe.1.2/oboe-core.owl#Standard"/>
        <owl:disjointWith rdf:resource="http://ecoinformatics.org/oboe/oboe.1.2/oboe-core.owl#UnitConversion"/>
        <rdfs:comment xml:lang="en">A MeasurementType describes the type of a Measurement in which the Measurement would follow the associated Protocol to record the value of the associated Characteristic of the associated Entity using the associated Standard.  Any of these associated properties may be omitted, in which case the MeasurementType is only constrained by the provided associations. A MeasurementType is a hypothetical construct, in that it is not associated with a particular instance of a Measurement.</rdfs:comment>
        <rdfs:label xml:lang="en">Measurement Type</rdfs:label>
    </owl:Class>
    


    <!-- http://ecoinformatics.org/oboe/oboe.1.2/oboe-core.owl#Observation -->

    <owl:Class rdf:about="http://ecoinformatics.org/oboe/oboe.1.2/oboe-core.owl#Observation">
        <rdfs:subClassOf>
            <owl:Restriction>
                <owl:onProperty rdf:resource="http://ecoinformatics.org/oboe/oboe.1.2/oboe-core.owl#ofEntity"/>
                <owl:someValuesFrom rdf:resource="http://ecoinformatics.org/oboe/oboe.1.2/oboe-core.owl#Entity"/>
            </owl:Restriction>
        </rdfs:subClassOf>
        <owl:disjointWith rdf:resource="http://ecoinformatics.org/oboe/oboe.1.2/oboe-core.owl#ObservationCollection"/>
        <owl:disjointWith rdf:resource="http://ecoinformatics.org/oboe/oboe.1.2/oboe-core.owl#Protocol"/>
        <owl:disjointWith rdf:resource="http://ecoinformatics.org/oboe/oboe.1.2/oboe-core.owl#Standard"/>
        <rdfs:comment rdf:datatype="http://www.w3.org/2001/XMLSchema#string"> An observation is an assertion that an entity (e.g., biological organisms, geographic locations, or environmental features, among others) was observed by an observer. An observation primarily serves to group a set of measurements together into a single &quot;observation event&quot;. Observations are often made within a broader context. The context of an observation is given by other observations, implying that an observed entity (and specifically each corresponding measurement) contextualizes another observed entity (and its corresponding measurements). For example, an observation associated with a location may serve as context for an observation associated with an organism. In this case, the observed characteristic values of the location (such as humidity) are assumed constant for the corresponding measurements of the organism.</rdfs:comment>
        <rdfs:label xml:lang="en">Observation</rdfs:label>
    </owl:Class>
    


    <!-- http://ecoinformatics.org/oboe/oboe.1.2/oboe-core.owl#ObservationCollection -->

    <owl:Class rdf:about="http://ecoinformatics.org/oboe/oboe.1.2/oboe-core.owl#ObservationCollection">
        <owl:disjointWith rdf:resource="http://ecoinformatics.org/oboe/oboe.1.2/oboe-core.owl#Protocol"/>
        <owl:disjointWith rdf:resource="http://ecoinformatics.org/oboe/oboe.1.2/oboe-core.owl#Standard"/>
        <rdfs:comment>An observation collection is a container for a set of observations.</rdfs:comment>
        <rdfs:label xml:lang="en">Observation Collection</rdfs:label>
    </owl:Class>
    


    <!-- http://ecoinformatics.org/oboe/oboe.1.2/oboe-core.owl#PrefixedUnit -->

    <owl:Class rdf:about="http://ecoinformatics.org/oboe/oboe.1.2/oboe-core.owl#PrefixedUnit">
        <rdfs:subClassOf rdf:resource="http://ecoinformatics.org/oboe/oboe.1.2/oboe-core.owl#Unit"/>
        <rdfs:subClassOf>
            <owl:Class>
                <owl:complementOf>
                    <owl:Restriction>
                        <owl:onProperty rdf:resource="http://ecoinformatics.org/oboe/oboe.1.2/oboe-core.owl#hasPrefixMultiplier"/>
                        <owl:hasValue rdf:datatype="http://www.w3.org/2001/XMLSchema#integer">0</owl:hasValue>
                    </owl:Restriction>
                </owl:complementOf>
            </owl:Class>
        </rdfs:subClassOf>
        <rdfs:subClassOf>
            <owl:Restriction>
                <owl:onProperty rdf:resource="http://ecoinformatics.org/oboe/oboe.1.2/oboe-core.owl#hasUnit"/>
                <owl:qualifiedCardinality rdf:datatype="http://www.w3.org/2001/XMLSchema#nonNegativeInteger">1</owl:qualifiedCardinality>
                <owl:onClass rdf:resource="http://ecoinformatics.org/oboe/oboe.1.2/oboe-core.owl#BaseUnit"/>
            </owl:Restriction>
        </rdfs:subClassOf>
        <rdfs:subClassOf>
            <owl:Restriction>
                <owl:onProperty rdf:resource="http://ecoinformatics.org/oboe/oboe.1.2/oboe-core.owl#hasPrefixMultiplier"/>
                <owl:someValuesFrom rdf:resource="http://www.w3.org/2001/XMLSchema#decimal"/>
            </owl:Restriction>
        </rdfs:subClassOf>
        <rdfs:comment>A prefixed unit consists of a base unit and a prefix integer value that serves as a multiplier. For example, a centimeter is a prefixed unit that combines a meter base unit and the prefix multiplier 0.01 such that one centimeter is equivalent to 0.01 meters.
</rdfs:comment>
    </owl:Class>
    


    <!-- http://ecoinformatics.org/oboe/oboe.1.2/oboe-core.owl#Protocol -->

    <owl:Class rdf:about="http://ecoinformatics.org/oboe/oboe.1.2/oboe-core.owl#Protocol">
        <rdfs:subClassOf>
            <owl:Restriction>
                <owl:onProperty>
                    <rdf:Description>
                        <owl:inverseOf rdf:resource="http://ecoinformatics.org/oboe/oboe.1.2/oboe-core.owl#usesProtocol"/>
                    </rdf:Description>
                </owl:onProperty>
                <owl:someValuesFrom rdf:resource="http://ecoinformatics.org/oboe/oboe.1.2/oboe-core.owl#Measurement"/>
            </owl:Restriction>
        </rdfs:subClassOf>
        <owl:disjointWith rdf:resource="http://ecoinformatics.org/oboe/oboe.1.2/oboe-core.owl#Standard"/>
        <rdfs:comment>A protocol is a procedure for generating or processing data.</rdfs:comment>
        <rdfs:label xml:lang="en">Protocol</rdfs:label>
    </owl:Class>
    


    <!-- http://ecoinformatics.org/oboe/oboe.1.2/oboe-core.owl#Standard -->

    <owl:Class rdf:about="http://ecoinformatics.org/oboe/oboe.1.2/oboe-core.owl#Standard">
        <rdfs:subClassOf>
            <owl:Restriction>
                <owl:onProperty>
                    <rdf:Description>
                        <owl:inverseOf rdf:resource="http://ecoinformatics.org/oboe/oboe.1.2/oboe-core.owl#usesStandard"/>
                    </rdf:Description>
                </owl:onProperty>
                <owl:someValuesFrom rdf:resource="http://ecoinformatics.org/oboe/oboe.1.2/oboe-core.owl#Measurement"/>
            </owl:Restriction>
        </rdfs:subClassOf>
        <rdfs:comment rdf:datatype="http://www.w3.org/2001/XMLSchema#string">A standard defines a reference for comparing or naming entities via a measurement. A standard can be defined intentionally (e.g., as in the case of units) or extensionally (by listing the values of the standard, e.g., for color this might be red, blue, yellow, etc).</rdfs:comment>
        <rdfs:label xml:lang="en">Standard</rdfs:label>
    </owl:Class>
    


    <!-- http://ecoinformatics.org/oboe/oboe.1.2/oboe-core.owl#Unit -->

    <owl:Class rdf:about="http://ecoinformatics.org/oboe/oboe.1.2/oboe-core.owl#Unit">
        <owl:equivalentClass>
            <owl:Class>
                <owl:unionOf rdf:parseType="Collection">
                    <rdf:Description rdf:about="http://ecoinformatics.org/oboe/oboe.1.2/oboe-core.owl#BaseUnit"/>
                    <rdf:Description rdf:about="http://ecoinformatics.org/oboe/oboe.1.2/oboe-core.owl#CompositeUnit"/>
                    <rdf:Description rdf:about="http://ecoinformatics.org/oboe/oboe.1.2/oboe-core.owl#DerivedUnit"/>
                    <rdf:Description rdf:about="http://ecoinformatics.org/oboe/oboe.1.2/oboe-core.owl#PrefixedUnit"/>
                </owl:unionOf>
            </owl:Class>
        </owl:equivalentClass>
        <rdfs:subClassOf rdf:resource="http://ecoinformatics.org/oboe/oboe.1.2/oboe-core.owl#Standard"/>
        <rdfs:comment>A unit is a standard quantification for physical measurements. A unit is either a base unit, a composite unit, or a derived unit.</rdfs:comment>
        <rdfs:label xml:lang="en">Unit</rdfs:label>
    </owl:Class>
    


    <!-- http://ecoinformatics.org/oboe/oboe.1.2/oboe-core.owl#UnitConversion -->

    <owl:Class rdf:about="http://ecoinformatics.org/oboe/oboe.1.2/oboe-core.owl#UnitConversion">
        <rdfs:subClassOf>
            <owl:Restriction>
                <owl:onProperty rdf:resource="http://ecoinformatics.org/oboe/oboe.1.2/oboe-core.owl#hasSourceUnit"/>
                <owl:someValuesFrom rdf:resource="http://ecoinformatics.org/oboe/oboe.1.2/oboe-core.owl#Unit"/>
            </owl:Restriction>
        </rdfs:subClassOf>
        <rdfs:subClassOf>
            <owl:Restriction>
                <owl:onProperty rdf:resource="http://ecoinformatics.org/oboe/oboe.1.2/oboe-core.owl#hasTargetUnit"/>
                <owl:someValuesFrom rdf:resource="http://ecoinformatics.org/oboe/oboe.1.2/oboe-core.owl#Unit"/>
            </owl:Restriction>
        </rdfs:subClassOf>
        <rdfs:subClassOf>
            <owl:Restriction>
                <owl:onProperty rdf:resource="http://ecoinformatics.org/oboe/oboe.1.2/oboe-core.owl#hasMultiplier"/>
                <owl:someValuesFrom rdf:resource="http://www.w3.org/2001/XMLSchema#decimal"/>
            </owl:Restriction>
        </rdfs:subClassOf>
        <rdfs:subClassOf>
            <owl:Restriction>
                <owl:onProperty rdf:resource="http://ecoinformatics.org/oboe/oboe.1.2/oboe-core.owl#hasOffset"/>
                <owl:someValuesFrom rdf:resource="http://www.w3.org/2001/XMLSchema#decimal"/>
            </owl:Restriction>
        </rdfs:subClassOf>
        <rdfs:comment>A unit conversion is a mapping from a source unit to a target unit via a multiplier and an offset value.</rdfs:comment>
        <rdfs:label xml:lang="en">Unit Conversion</rdfs:label>
    </owl:Class>
    


    <!-- 
    ///////////////////////////////////////////////////////////////////////////////////////
    //
    // Rules
    //
    ///////////////////////////////////////////////////////////////////////////////////////
     -->

    <rdf:Description rdf:about="urn:swrl#c">
        <rdf:type rdf:resource="http://www.w3.org/2003/11/swrl#Variable"/>
    </rdf:Description>
    <rdf:Description rdf:about="urn:swrl#e">
        <rdf:type rdf:resource="http://www.w3.org/2003/11/swrl#Variable"/>
    </rdf:Description>
    <rdf:Description rdf:about="urn:swrl#o">
        <rdf:type rdf:resource="http://www.w3.org/2003/11/swrl#Variable"/>
    </rdf:Description>
    <rdf:Description rdf:about="urn:swrl#m">
        <rdf:type rdf:resource="http://www.w3.org/2003/11/swrl#Variable"/>
    </rdf:Description>
    <rdf:Description>
        <rdf:type rdf:resource="http://www.w3.org/2003/11/swrl#Imp"/>
        <swrl:body>
            <rdf:Description>
                <rdf:type rdf:resource="http://www.w3.org/2003/11/swrl#AtomList"/>
                <rdf:first>
                    <rdf:Description>
                        <rdf:type rdf:resource="http://www.w3.org/2003/11/swrl#IndividualPropertyAtom"/>
                        <swrl:propertyPredicate rdf:resource="http://ecoinformatics.org/oboe/oboe.1.2/oboe-core.owl#characteristicFor"/>
                        <swrl:argument1 rdf:resource="urn:swrl#c"/>
                        <swrl:argument2 rdf:resource="urn:swrl#e"/>
                    </rdf:Description>
                </rdf:first>
                <rdf:rest>
                    <rdf:Description>
                        <rdf:type rdf:resource="http://www.w3.org/2003/11/swrl#AtomList"/>
                        <rdf:first>
                            <rdf:Description>
                                <rdf:type rdf:resource="http://www.w3.org/2003/11/swrl#IndividualPropertyAtom"/>
                                <swrl:propertyPredicate rdf:resource="http://ecoinformatics.org/oboe/oboe.1.2/oboe-core.owl#hasMeasurement"/>
                                <swrl:argument1 rdf:resource="urn:swrl#o"/>
                                <swrl:argument2 rdf:resource="urn:swrl#m"/>
                            </rdf:Description>
                        </rdf:first>
                        <rdf:rest>
                            <rdf:Description>
                                <rdf:type rdf:resource="http://www.w3.org/2003/11/swrl#AtomList"/>
                                <rdf:first>
                                    <rdf:Description>
                                        <rdf:type rdf:resource="http://www.w3.org/2003/11/swrl#IndividualPropertyAtom"/>
                                        <swrl:propertyPredicate rdf:resource="http://ecoinformatics.org/oboe/oboe.1.2/oboe-core.owl#ofCharacteristic"/>
                                        <swrl:argument1 rdf:resource="urn:swrl#m"/>
                                        <swrl:argument2 rdf:resource="urn:swrl#c"/>
                                    </rdf:Description>
                                </rdf:first>
                                <rdf:rest rdf:resource="http://www.w3.org/1999/02/22-rdf-syntax-ns#nil"/>
                            </rdf:Description>
                        </rdf:rest>
                    </rdf:Description>
                </rdf:rest>
            </rdf:Description>
        </swrl:body>
        <swrl:head>
            <rdf:Description>
                <rdf:type rdf:resource="http://www.w3.org/2003/11/swrl#AtomList"/>
                <rdf:first>
                    <rdf:Description>
                        <rdf:type rdf:resource="http://www.w3.org/2003/11/swrl#IndividualPropertyAtom"/>
                        <swrl:propertyPredicate rdf:resource="http://ecoinformatics.org/oboe/oboe.1.2/oboe-core.owl#ofEntity"/>
                        <swrl:argument1 rdf:resource="urn:swrl#o"/>
                        <swrl:argument2 rdf:resource="urn:swrl#e"/>
                    </rdf:Description>
                </rdf:first>
                <rdf:rest rdf:resource="http://www.w3.org/1999/02/22-rdf-syntax-ns#nil"/>
            </rdf:Description>
        </swrl:head>
    </rdf:Description>
    <rdf:Description>
        <rdf:type rdf:resource="http://www.w3.org/2003/11/swrl#Imp"/>
        <swrl:body>
            <rdf:Description>
                <rdf:type rdf:resource="http://www.w3.org/2003/11/swrl#AtomList"/>
                <rdf:first>
                    <rdf:Description>
                        <rdf:type rdf:resource="http://www.w3.org/2003/11/swrl#IndividualPropertyAtom"/>
                        <swrl:propertyPredicate rdf:resource="http://ecoinformatics.org/oboe/oboe.1.2/oboe-core.owl#hasMeasurement"/>
                        <swrl:argument1 rdf:resource="urn:swrl#o"/>
                        <swrl:argument2 rdf:resource="urn:swrl#m"/>
                    </rdf:Description>
                </rdf:first>
                <rdf:rest>
                    <rdf:Description>
                        <rdf:type rdf:resource="http://www.w3.org/2003/11/swrl#AtomList"/>
                        <rdf:first>
                            <rdf:Description>
                                <rdf:type rdf:resource="http://www.w3.org/2003/11/swrl#IndividualPropertyAtom"/>
                                <swrl:propertyPredicate rdf:resource="http://ecoinformatics.org/oboe/oboe.1.2/oboe-core.owl#ofCharacteristic"/>
                                <swrl:argument1 rdf:resource="urn:swrl#m"/>
                                <swrl:argument2 rdf:resource="urn:swrl#c"/>
                            </rdf:Description>
                        </rdf:first>
                        <rdf:rest>
                            <rdf:Description>
                                <rdf:type rdf:resource="http://www.w3.org/2003/11/swrl#AtomList"/>
                                <rdf:first>
                                    <rdf:Description>
                                        <rdf:type rdf:resource="http://www.w3.org/2003/11/swrl#IndividualPropertyAtom"/>
                                        <swrl:propertyPredicate rdf:resource="http://ecoinformatics.org/oboe/oboe.1.2/oboe-core.owl#ofEntity"/>
                                        <swrl:argument1 rdf:resource="urn:swrl#o"/>
                                        <swrl:argument2 rdf:resource="urn:swrl#e"/>
                                    </rdf:Description>
                                </rdf:first>
                                <rdf:rest rdf:resource="http://www.w3.org/1999/02/22-rdf-syntax-ns#nil"/>
                            </rdf:Description>
                        </rdf:rest>
                    </rdf:Description>
                </rdf:rest>
            </rdf:Description>
        </swrl:body>
        <swrl:head>
            <rdf:Description>
                <rdf:type rdf:resource="http://www.w3.org/2003/11/swrl#AtomList"/>
                <rdf:first>
                    <rdf:Description>
                        <rdf:type rdf:resource="http://www.w3.org/2003/11/swrl#IndividualPropertyAtom"/>
                        <swrl:propertyPredicate rdf:resource="http://ecoinformatics.org/oboe/oboe.1.2/oboe-core.owl#characteristicFor"/>
                        <swrl:argument1 rdf:resource="urn:swrl#c"/>
                        <swrl:argument2 rdf:resource="urn:swrl#e"/>
                    </rdf:Description>
                </rdf:first>
                <rdf:rest rdf:resource="http://www.w3.org/1999/02/22-rdf-syntax-ns#nil"/>
            </rdf:Description>
        </swrl:head>
    </rdf:Description>
</rdf:RDF>



<!-- Generated by the OWL API (version 4.2.5.20160517-0735) https://github.com/owlcs/owlapi -->

